examples/bytestring/prims_verif.v
@@ -1,0 +1,30 @@
+Require Import VeriFFI.examples.bytestring.prims.
+Require Import ZArith.
+Require Import Psatz.
+Require Import CertiGraph.CertiGC.spatial_gcgraph.
+
+Require Import VeriFFI.examples.bytestring.specs.
+
+Lemma body_pack:
+  semax_body Vprog Gprog f_pack pack_spec.
+Proof.
+ start_function'.
+ forward.
+ forward.
+ change (Tpointer _ _) with int_or_ptr_type. simpl snd.
+ unfold full_gc.
+ unfold before_gc_thread_info_rep.
+ Intros.
+ limited_change_compspecs CompSpecs.
+ forward.
+ forward.
+ forward.
+ forward.
+ Admitted.
+
+(* REMAINDER OF THIS FILE DUPLICATED FROM examples/uint63nat/prims_verif.v *)
+
+#[export] Instance CCE: change_composite_env env_graph_gc.CompSpecs CompSpecs.
+make_cs_preserve env_graph_gc.CompSpecs CompSpecs.
+Defined.
+
