examples/bytestring/specs.v
@@ -1,0 +1,65 @@
+Require Import VeriFFI.examples.bytestring.prog.
+Require Import ZArith.
+Require Import Psatz.
+Require Export VeriFFI.verification.specs_general.
+Require Export VeriFFI.generator.Rep.
+
+Import Ascii.
+Import Coq.Strings.String.
+
+#[local] Obligation Tactic := gen.
+MetaCoq Run (gen_for ascii).
+MetaCoq Run (gen_for string).
+
+
+Require Export VST.floyd.proofauto.
+Require Export CertiGraph.CertiGC.GCGraph.
+Export spatial_gcgraph.
+From VeriFFI Require Export library.base_representation library.meta verification.graph_add verification.specs_library.
+
+Require Import VeriFFI.examples.bytestring.prog.
+Require Export VeriFFI.examples.bytestring.model.
+Require Export VeriFFI.examples.bytestring.prims. 
+
+
+#[export] Instance CompSpecs : compspecs. make_compspecs prog. Defined.
+
+#[export] Instance CCE1: change_composite_env env_graph_gc.CompSpecs CompSpecs.
+make_cs_preserve env_graph_gc.CompSpecs CompSpecs.
+Defined.
+
+
+MetaCoq Run (desc_gen EmptyString).
+MetaCoq Run (desc_gen String).
+MetaCoq Run (desc_gen Ascii).
+
+Definition make_Coq_Strings_String_string_EmptyString_spec : ident * funspec :=
+    DECLARE _make_Coq_Strings_String_string_EmptyString
+          (alloc_make_spec_general (@desc _ EmptyString _) 0). 
+
+Definition alloc_make_Coq_Strings_String_string_String_spec : ident * funspec :=
+    DECLARE _alloc_make_Coq_Strings_String_string_String
+          (alloc_make_spec_general (@desc _ String _) 2).     
+
+Definition alloc_make_Coq_Strings_Ascii_ascii_Ascii_spec : ident * funspec :=
+    DECLARE _alloc_make_Coq_Strings_Ascii_ascii_Ascii
+          (alloc_make_spec_general (@desc _ Ascii _) 8). 
+
+
+Definition pack_spec : ident * funspec :=
+  fn_desc_to_funspec Bytestring_Proofs.pack_desc.
+
+Definition unpack_spec : ident * funspec :=
+  fn_desc_to_funspec Bytestring_Proofs.unpack_desc.
+
+Definition append_spec : ident * funspec :=
+  fn_desc_to_funspec Bytestring_Proofs.append_desc.
+
+
+Definition Vprog : varspecs. mk_varspecs prog. Defined.
+Definition Gprog := [ make_Coq_Strings_String_string_EmptyString_spec;
+                      alloc_make_Coq_Strings_String_string_String_spec;
+                      alloc_make_Coq_Strings_Ascii_ascii_Ascii_spec;
+                      gc_spec.garbage_collect_spec
+                      (* _call, call_spec *)
+                      ] .
